examples/xor_swap_proofs.v
@@ -4,7 +4,6 @@ From Coq          Require Import String.
 From Coq          Require Import Vectors.Vector.
 From CryptolToCoq Require Import SAWCoreScaffolding.
 From CryptolToCoq Require Import SAWCoreVectorsAsCoqVectors.
-From Records      Require Import Records.
 
 From CryptolToCoq Require Import SAWCorePrelude.
 From CryptolToCoq Require Import CompMExtra.
